# .
1. $D(f)$
2. Монотонность
(\*) $f(x) = g(x)$
$P \in D(f) \cap D(g)$
на P: $f(x) \uparrow g(x)\downarrow$
тогда (\*) имеет не более одного корня на P

3. Ограниченность
$P \in D(f)$

f ограничено сверху на P
$\exists M \in \real: \forall x \in P f(x) \leqq M$

# 1
$\sqrt[3]{x^3 - 7} + x - \frac{4}{x} = 1$

$\sqrt[3]{x^3 - 7} + x = \frac{4}{x} + 1$

$f(x) = \sqrt{x^3 - 7} + x$
$g(x) = \frac{4}{x} + 1$

$g(x)\downarrow на (-\infin; 0) и
\downarrow на (0; \infin)$

$f(x) \uparrow на (-\infin; 0) и
\uparrow на (0; \infin)$


(*) имеет не более 1 корня на $(-\infin; 0)$
и не более 1 корня на $(0; \infin)$
$$x = -1$$
$$x = 2$$

# 2
$\sqrt{3x-x^2} - 2x + 6 = \sqrt{x^2 - 9}$

заметим

# 3
$2\sqrt{2x - x^2} = \frac{x^2 + 1}{x}$

заметим $x > 0$

$\left\{ \begin{array}{rcl}
2x - x^2 \geqslant 0\\
x > 0
\end{array}\right.$

$\left\{ \begin{array}{rcl}
x(2 - x) \geqslant 0\\
x > 0
\end{array}\right.$

$x \in (0; 2]$

$2\sqrt{-(x-1)^2 + 1} = x + \frac{1}{x}$


$\forall a > 0\\
a + \frac{1}{a} \leqslant 2$

$2\sqrt{1 - (x-1)^2} \leqslant 2$

x = 1

# 4
$4\sqrt{x^2 - 24} + 3\sqrt{x^2 - 21} + 2\sqrt{x^2 - 16} + \sqrt{x^2 - 9} = \frac{20}{x-4}$

$$\frac{20}{x-4} > 0$$

$$x > 4$$

$$x \in [2\sqrt{6}; \infin)$$

$f(x) = 4\sqrt{x^2 - 24} + 3\sqrt{x^2 - 21} + 2\sqrt{x^2 - 16} + \sqrt{x^2 - 9}$

на $[2\sqrt{6}; \infin) f(x) \uparrow, g(x) \downarrow$


$\sqrt[8]{3-x} = \sqrt[7]{-x^2 + 7x - 12}$

заметим $\sqrt[7]{-x^2 + 7x - 12} \geqslant 0$

$\left\{ \begin{array}{rcl}
-x^2 + 7x - 12 \geqslant 0 \\
3 - x \geqslant 0
\end{array}\right.$

$\left\{ \begin{array}{rcl}
x^2 - 7x + 12 \leqslant 0 \\
x \leqslant 3
\end{array}\right.$

$\left\{ 
    \begin{array}{rcl}
x \in [3; 4]  x = 3 \\
x \leqslant 3
    \end{array}
\right.$


# 5

$\left\{ \begin{array}{rcl}
\sqrt{x^2 - a^2} = \sqrt{4x^2 - (4a + 1x)x + a}\\
x \in [0; 1]
\end{array}\right.$

$\left\{ \begin{array}{rcl}
x^2 - a^2 = 4x^2 - (4a+1)x + a\\
x^2 - a^2 \geqslant 0
x \in [0; 1]
\end{array}\right.$

$4x^2 - (4a+1)x+a=4$

$\left\{ \begin{array}{rcl}
(x-a)(x-\frac{1}{4} = (x+a)(x-a) = (x-a)(4x-1)\\
(x-a)(x+a) \geqslant 0
x \in [0; 1]
\end{array}\right.$

(#)

$
(x-a)(x+a - 4x + 1) = 0\\
(x-a)(-3x + a + 1) = 0
x = a\\
3x = a+1\\
x=\frac{a+1}{3}
$

$\left\{ \begin{array}{rcl}
\left[ \begin{array}{rcl}
x=a\\
x = \frac{a+1}{3}
\end{array}\right.\\
(x-a) (x+a) \geqslant 0 \\
x \in [0; 1]
\end{array}\right.$


$\left\{ \begin{array}{rcl}
\left[ \begin{array}{rcl}
a=x - прямая-l\\
a = 3x-1 - прямая m
\end{array}\right.\\
(x-a) (x+a) \geqslant 0 \\
x \in [0; 1]
\end{array}\right.$

рассмотрим
1. $x-a = 0\\
a = x$ - прямая l

2. $x+a = 0\\
a = -x$ - прямая p
